minterop.fst
@@ -36,18 +36,27 @@ instance ml_check_type : ml check_type = { mldummy = () }
 
 exception Contract_failure
 class exportable (t : Type) = { etype : Type; export : t -> etype; ml_etype : ml etype }
-class importable (t : Type) = { itype : Type; import : itype -> M4 t; ml_itype : ml itype }
+class importable (t : Type) = { itype : Type; import : itype -> option t; ml_itype : ml itype }
+class exn_importable (t : Type) = { eitype : Type; exn_import : eitype -> M4 t; ml_eitype : ml eitype }
 
-let mk_exportable (#t1 t2 : Type) {|ml t2|} (exp : t1 -> t2) : exportable t1 =
+let mk_exportable (#t1 t2 : Type) {| ml t2 |} (exp : t1 -> t2) : exportable t1 =
   { etype = t2; export = exp;  ml_etype = solve }
-let mk_importable (t1 #t2 : Type) {|ml t1|} (imp : t1 -> M4 t2) : importable t2 =
-  { itype = t1; import = imp;  ml_itype = solve }
+let mk_importable (t1 #t2 : Type) {| ml t1 |} (imp : t1 -> option t2) : importable t2 =
+  { itype = t1; import = imp; ml_itype = solve }
+let mk_exn_importable (t1 #t2 : Type) {| ml t1 |} (imp : t1 -> M4 t2) : exn_importable t2 =
+  { eitype = t1; exn_import = imp; ml_eitype = solve }
 
 instance ml_exportable (#t : Type) (d : exportable t) : ml (d.etype) = d.ml_etype
 instance ml_importable (#t : Type) (d : importable t) : ml (d.itype) = d.ml_itype
 
-instance exportable_ml t {| ml t|} : exportable t = mk_exportable t (fun x -> x)
-instance importable_ml t {| ml t|} : importable t = mk_importable t (fun x -> x)
+instance exportable_ml t {| ml t |} : exportable t = mk_exportable t (fun x -> x)
+instance importable_ml t {| ml t |} : importable t = mk_importable t (fun x -> Some x)
+
+instance exn_importable_importable t {| d:importable t |} : exn_importable t =
+  mk_exn_importable d.itype (fun x -> 
+    (match import x with
+    | Some x -> x
+    | None -> raise Contract_failure) <: M4 t)
 
 instance exportable_refinement t {| d:exportable t |} (p : t -> Type0)  : exportable (x:t{p x})
 = mk_exportable (d.etype) export // TODO: Eta expanding causes type error
@@ -66,11 +75,11 @@ instance importable_refinement
     importable (x:t{rp x}) = 
   mk_importable (d.itype)
     (fun (x:d.itype) ->
-      let x : t = import x in
-      (if check #t #rp x then x
-       else M4.raise Contract_failure) <: M4 (x:t{rp x}))
+      (match import x with
+      | Some x -> if check #t #rp x then Some x else None
+      | None -> None) <: option (x:t{rp x}))
 
-let test_refinement () : M4 (y:int{y = 5}) = import 5
+let test_refinement () : M4 (y:int{y = 5}) = exn_import 5
 
 (* TODO: quite a few type annotations needed above *)
 
@@ -78,23 +87,26 @@ instance exportable_pair t1 t2 {| d1:exportable t1 |} {| d2:exportable t2 |} : e
   mk_exportable (d1.etype * d2.etype) (fun (x,y) -> (export x, export y))
 
 instance importable_pair t1 t2 {| d1:importable t1 |} {| d2:importable t2 |} : importable (t1 * t2) =
-  mk_importable (d1.itype * d2.itype) (fun (x,y) -> (import x, import y) <: M4 (t1 * t2))
+  mk_importable (d1.itype * d2.itype) (fun (x,y) -> 
+    (match (import x, import y) with
+    | (Some x, Some y) -> Some (x, y)
+    | _ -> None) <: option (t1 * t2))
 
 instance importable_dpair_refined t1 t2 (p:t1 -> t2 -> Type0)
   {| d1:importable t1 |} {| d2:importable t2 |} {| d3:checkable2 p |} : importable (x:t1 & y:t2{p x y}) =
   mk_importable (d1.itype & d2.itype) #(x:t1 & y:t2{p x y})
     (fun ((x', y')) ->
-        let (x : t1) = import x' in
-        let (y : t2) = import y' in
-        (if check2 #t1 #t2 #p x y then (| x, y |) 
-        else M4.raise Contract_failure) <: (x:t1 & y:t2{p x y}))
+      (match (import x', import y') with
+       | (Some x, Some y) ->
+               if check2 #t1 #t2 #p x y then Some (| x, y |) else None
+       | _ -> None) <: option (x:t1 & y:t2{p x y}))
 
-let test_dpair_refined () : M4 (a:int & b:int{b = a + 1}) = import (10, 11)
+let test_dpair_refined () : M4 (a:int & b:int{b = a + 1}) = exn_import (10, 11)
 
 // A typed term in an untyped context
 instance exportable_arrow t1 t2 {| d1:importable t1 |} {| d2:exportable t2 |} : exportable (t1 -> Tot t2)  =
   mk_exportable (d1.itype -> M4 d2.etype)
-    (fun (f:(t1 -> t2)) -> (fun (x:d1.itype) -> export (f (import x)) <: M4 d2.etype))
+    (fun (f:(t1 -> t2)) -> (fun (x:d1.itype) -> export (f (exn_import x)) <: M4 d2.etype))
   
 // instance exportable_exarrow t1 t2 {| d1:importable t1 |} {| d2:exportable t2 |} : exportable (t1 -> Ex t2)  =
 //   mk_exportable (d1.itype -> M4 d2.etype)
@@ -102,26 +114,27 @@ instance exportable_arrow t1 t2 {| d1:importable t1 |} {| d2:exportable t2 |} : 
 
 instance exportable_mlarrow t1 t2 {| d1:importable t1 |} {| d2:exportable t2 |} : exportable (t1 -> M4 t2)  =
   mk_exportable (d1.itype -> M4 d2.etype)
-    (fun (f:(t1 -> M4 t2)) -> (fun (x:d1.itype) -> export (f (import x)) <: M4 d2.etype))
+    (fun (f:(t1 -> M4 t2)) -> (fun (x:d1.itype) -> export (f (exn_import x)) <: M4 d2.etype))
 
 // An untyped term in a typed context
 instance importable_mlarrow t1 t2 {| d1:exportable t1 |} {| d2:importable t2 |} : importable (t1 -> M4 t2)  =
   mk_importable (d1.etype -> M4 d2.itype)
-    (fun (f:(d1.etype -> M4 d2.itype)) -> (fun (x:t1) -> import (f (export x)) <: M4 t2))
+    (fun (f:(d1.etype -> M4 d2.itype)) -> 
+      Some (fun (x:t1) -> exn_import (f (export x)) <: M4 t2))
   
 // Example trueish
 let trueish (x:int{x >= 0}) : bool = true
-let trueish' (x:int) : M4 bool = (trueish (import x))
+let trueish' (x:int) : M4 bool = (trueish (exn_import x))
 let trueish'' : int -> M4 bool = export trueish
 
 instance importable_darrow_refined t1 t2 (p:t1->t2->Type0)
   {| d1:ml t1 |} {| d2:ml t2 |} {| d3:checkable2 p |} : importable (x:t1 -> M4 (y:t2{p x y})) =
   mk_importable (t1 -> M4 t2) #(x:t1 -> M4 (y:t2{p x y}))
     (fun (f:(t1 -> M4 t2)) -> 
-      (fun (x:t1) -> 
+      let f':(x:t1 -> M4 (y:t2{p x y})) = (fun (x:t1) -> 
         let y : t2 = f x in
         (if check2 #t1 #t2 #p x y then y 
-         else M4.raise Contract_failure) <: M4 (y:t2{p x y})))
+         else M4.raise Contract_failure) <: M4 (y:t2{p x y})) in Some f')
 
 // Example incr
 
@@ -130,7 +143,7 @@ let incr (x:int) : int = x + 1
 let incr2 : int -> M4 int = incr
 
 let p x y : bool = (y = x + 1)
-let incr'' (x:int) : M4 (y:int{p x y}) = import (incr x)
+let incr'' (x:int) : M4 (y:int{p x y}) = exn_import (incr x)
 
 // val incr' : unit -> M4 ((x:int) -> M4 (y:int{p x y}))
 // let incr' () = 
@@ -142,7 +155,7 @@ instance exportable_purearrow_spec t1 t2 (pre : t1 -> Type0) (post : t1 -> t2 ->
   mk_exportable (d1.itype -> M4 d2.etype)
     (fun (f:(x:t1 -> Pure t2 (pre x) (post x))) ->
       (fun (x:d1.itype) ->
-        let x : t1 = import x in
+        let x : t1 = exn_import x in
         (if check #t1 #pre x then (
           export (f x)
         ) else raise Contract_failure) <: M4 d2.etype))
@@ -156,24 +169,28 @@ let incrs2  : (x:int) -> Pure int (x > 0) (fun (y:int) -> y = x + 1) = fun x -> 
 let incrs2' : int -> M4 int = export incrs2
 
 let _export_IOStHist_arrow_spec #t1 #t2 
-  {| d1:ml t1 |} {| d2:exportable t2 |}
+  {| d1:importable t1 |} {| d2:exportable t2 |}
   (pre : t1 -> events_trace -> Type0)
   {| checkable2 pre |}
   (post : t1 -> events_trace -> maybe (events_trace * t2) -> events_trace -> Type0)
   (f:(x:t1 -> IOStHist t2 (pre x) (post x))) : 
-  Tot (t1 -> M4 d2.etype) =
-    (fun (x:t1) ->
+  Tot (d1.itype -> M4 d2.etype) =
+    (fun (x:d1.itype) ->
+      match import x with
+      | Some x -> (
         if (check2 #t1 #events_trace #pre x []) then (
             let tree = reify (f x) (fun r le -> post x [] r le) in
             export (M4wp?.reflect (fun _ -> iost_to_io (tree [])) <: M4wp t2 (fun p -> forall res. p res))
         ) else M4.raise Contract_failure)
+      | None -> M4.raise Contract_failure)
+        
 
 instance exportable_IOStHist_arrow_spec t1 t2 (pre : t1 -> events_trace -> Type0) (post : t1 -> events_trace -> maybe (events_trace * t2) -> events_trace -> Type0)
   {| d1:importable t1 |} {| d2:exportable t2 |} {| d4:checkable2 pre |} : exportable ((x:t1) -> IOStHist t2 (pre x) (post x)) = 
   mk_exportable (d1.itype -> M4 d2.etype)
     (fun (f:(x:t1 -> IOStHist t2 (pre x) (post x))) ->
       (fun (x:d1.itype) ->
-        let x : t1 = import x in
+        let x : t1 = exn_import x in
         let s0 : events_trace = M4.get_history () in
         (if check2 #t1 #events_trace #pre x s0 then (
           let tree = reify (f x) (fun r le -> post x s0 r le) in
@@ -229,10 +246,10 @@ instance importable_M4_arrow_spec t1 t2 {| d1:exportable t1 |} {| d2:ml t2 |} :
   importable(pi:check_type -> t1 -> GIO t2 pi) =
   mk_importable (d1.etype -> M4 t2) #(pi:check_type -> t1 -> GIO t2 pi)
     (fun (f:(d1.etype -> M4 t2)) ->
-      (fun (pi:check_type) (x:t1) ->
+      let f' : (pi:check_type -> t1 -> GIO t2 pi) = (fun (pi:check_type) (x:t1) ->
         let x : d1.etype = export x in
         let tree = reify (f x) (fun r -> True) in
-        _import_M4_to_GIO #t2 tree pi <: GIO t2 pi))
+        _import_M4_to_GIO #t2 tree pi <: GIO t2 pi) in Some f')
 
 val allowed_file : string -> bool
 let allowed_file fnm = match fnm with
@@ -270,8 +287,8 @@ let m4_cmd (cmd:io_cmds) (argz: args cmd) : M4 (res cmd) =
 let plugin1 : file_descr -> M4 unit = fun fd ->
   m4_cmd Close fd
 
-// val plugin1_g : (pi:check_type) -> file_descr -> GIO unit pi 
-// let plugin1_g = import plugin1
+// val plugin1_g : unit -> M4 ((pi:check_type) -> file_descr -> GIO unit pi)
+// let plugin1_g () = exn_import plugin1
 
 // let sdx () : GIO unit pi = 
 //   webserver (plugin1_g)
